Checkpoint.

AddLoop.v
@@ -1,55 +1,150 @@
-Require Import Omega String ZArith Vector.
+From Coq Require Import ZArith.ZArith Strings.String.
+Require Import mathcomp.ssreflect.ssreflect.
+From mathcomp Require Import ssrfun ssrbool eqtype ssrnat seq fintype tuple.
 
-Local Open Scope vector_scope.
-Local Open Scope Z_scope.
+Set Implicit Arguments.
+Unset Strict Implicit.
+Import Prenex Implicits.
+Import Ascii.
 
-Import VectorNotations.
+Definition BITS n := n.-tuple bool.
+Notation eta_expand x := (fst x, snd x).
+Definition splitlsb {n} (p: BITS n.+1): BITS n*bool := (behead_tuple p, thead p).
+Definition joinlsb {n} (pair: BITS n*bool) : BITS n.+1 := cons_tuple pair.2 pair.1.
+Notation "'nilB'" := (nil_tuple _).
+Coercion singleBit b : BITS 1 := joinlsb (nilB, b).
 
-Inductive reg : Set := r3 | r6 | r8.
-Definition reg_dec : forall r r' : reg, {r = r'} + {r <> r'}.
+(* Extend by one bit at the most significant bit. Again, signExtend 1 n does not work
+   because BITS (n+1) is not definitionally equal to BITS n.+1  *)
+Fixpoint joinmsb {n} : bool * BITS n -> BITS n.+1 :=
+  if n is _.+1
+  then fun p => let (hibit, p) := p in
+                let (p,b) := splitlsb p in joinlsb (joinmsb (hibit, p), b)
+  else fun p => joinlsb (nilB, p.1).
+Definition joinmsb0 {n} (p: BITS n) : BITS n.+1 := joinmsb (false,p).
+
+(* Special case: split at the most significant bit.
+   split 1 n doesn't work because it requires BITS (n+1) not BITS n.+1 *)
+Fixpoint splitmsb {n} : BITS n.+1 -> bool * BITS n :=
+  if n is _.+1
+  then fun p => let (p,b) := splitlsb p in let (c,r) := splitmsb p in (c,joinlsb(r,b))
+  else fun p => let (p,b) := splitlsb p in (b,p).
+Arguments splitmsb : simpl never.
+
+Definition dropmsb {n} (p: BITS n.+1) := (splitmsb p).2.
+
+Definition fullAdder carry b1 b2 : bool * bool :=
+    match carry, b1, b2 with
+    | false, false, false => (false, false)
+    | true, false, false | false, true, false | false, false, true => (false, true)
+    | true, true, false | false, true, true | true, false, true => (true, false)
+    | true, true, true => (true, true)
+    end.
+
+(* Add with carry, producing a word one bit larger than the inputs *)
+Fixpoint adcBmain n carry : BITS n -> BITS n -> BITS n.+1 :=
+  if n is _.+1 then
+    fun p1 p2 => let (p1,b1) := eta_expand (splitlsb p1) in
+                 let (p2,b2) := eta_expand (splitlsb p2) in
+                 let (carry',b) := fullAdder carry b1 b2 in
+                   joinlsb (adcBmain carry' p1 p2, b)
+  else fun _ _ => singleBit carry.
+Arguments adcBmain n carry a b : simpl never.
+
+Definition adcB {n} carry (p1 p2: BITS n) := splitmsb (adcBmain carry p1 p2).
+
+Fixpoint fromNat {n} m : BITS n :=
+  if n is _.+1
+  then joinlsb (fromNat m./2, odd m)
+  else nilB.
+Notation "# m" := (fromNat m) (at level 0).
+Arguments fromNat n m : simpl never.
+
+Definition toNat {n} (p: BITS n) := foldr (fun (b:bool) n => b + n.*2) 0 p.
+
+Definition charToBit c : bool := ascii_dec c "1".
+
+Fixpoint fromBin s : BITS (length s) :=
+  if s is String c s
+  then joinmsb (charToBit c, fromBin s) else #0.
+
+Notation "#b y" := (fromBin y) (at level 0).
+
+Check #0.
+Check #b"0111".
+
+Check adcBmain false.
+Definition a1 := #b"111".
+Definition a2 := #b"001".
+Compute (toNat a1).
+Compute (toNat a2).
+Definition res := (adcBmain false a1 a2).
+Compute (toNat res).
+Compute (fst (splitmsb res)).
+Compute (splitmsb res).
+Example e1 : (adcBmain false #b"01" #b"01") = (fromNat 2).
+Proof.
+  simpl. unfold adcBmain. unfold fullAdder. simpl.
+  unfold joinlsb. simpl. unfold cons_tuple. reflexivity.
+Qed.
+
+
+Inductive Reg : Set := r1 | r2 | r3 | r6 | r8.
+Definition reg_dec : forall r r' : Reg, {r = r'} + {r <> r'}.
 Proof. intros. decide equality. Defined.
 
-Inductive bitvec (n : nat): Type :=
-| BEndian (v: Vector.t bool n)
-| LEndian (v: Vector.t bool n).
+Definition total_map (A : Type) := Reg -> A.
+Definition t_empty {A : Type} (v : A) : total_map A := (fun _ => v).
+Definition beq_reg x y :=
+  if reg_dec x y then true else false.
+Definition t_update {A : Type} (m : total_map A) (x : Reg) (v : A) :=
+  fun x' => if (beq_reg x x') then v else m x'.
+Theorem reg_dec_refl : forall x, true  = reg_dec x x.
+Proof.
+  intros x. induction x; reflexivity.
+Qed.
+Lemma t_update_eq : forall A (m : total_map A) x v,
+  (t_update m x v) x = v.
+Proof. intros. unfold t_update.
+       unfold beq_reg.
+       rewrite <- reg_dec_refl. reflexivity.
+Qed.
+Theorem beq_reg_true_iff : forall x y,
+  beq_reg x y = true <-> x = y.
+Proof.
+  intros [] []; split; try reflexivity; try intro H; inversion H.
+Qed.
+Theorem not_true_is_false : forall b : bool,
+  b <> true -> b = false.
+Proof.
+  intros [] H.
+  - unfold not in H. exfalso. apply H. reflexivity. reflexivity.
+Qed.
+Lemma not_true_iff_false : forall b,
+  b <> true <-> b = false.
+Proof.
+  intros b. split.
+  - apply not_true_is_false.
+  - intros H. rewrite H. intros H'. inversion H'.
+Qed.
+Theorem beq_reg_false_iff : forall x y,
+    beq_reg x y = false <-> x <> y.
+    intros x y. rewrite <- beq_reg_true_iff.
+  rewrite not_true_iff_false. reflexivity.
+Qed.
+Theorem t_update_neq : forall (X : Type) v x1 x2 (m : total_map X),
+  x1 <> x2 -> (t_update m x1 v) x2 = m x2.
+Proof.
+  intros. unfold t_update.  apply beq_reg_false_iff in H. 
+  rewrite H. reflexivity.
+Qed.
 
-Fixpoint bitvecstr {n} (lendian : bool) (v : Vector.t bool n) : string :=
-  match lendian, v with
-  | false, true :: tl => "1" ++ bitvecstr lendian tl
-  | false, false :: tl => "0" ++ bitvecstr lendian tl
-  | true, true :: tl =>  bitvecstr lendian tl ++ "1"
-  | true, false :: tl => bitvecstr lendian tl ++ "0"
-  | _, [] => ""
-  end.
-
-Definition bvstr {n} (bv : bitvec n) : string :=
-  match bv with
-  | BEndian _ v => bitvecstr false v
-  | LEndian _ v => bitvecstr true v
-  end.
-
-Definition ex1 := BEndian 4 ([true; true; true; false]).
-Compute bvstr ex1.
-Definition ex2 := LEndian 4 ([true; true; true; false]).
-Compute bvstr ex2.
-
-(*
-Fixpoint add_bv {n} (v1: bitvec n) (v2: bitvec n) : bitvec n :=
-  match (bvunwrap v1), (bvunwrap v2) with
-  | , _ => v1
-  end.
-*)
-
-Definition total_map (A : Type) := reg -> A.
- Definition t_empty {A : Type} (v : A) : total_map A := (fun _ => v).
-Definition t_update {A : Type} (m : total_map A) (x : reg) (v : A) :=
-  fun x' => if (reg_dec x x') then v else m x'.
-
-Definition reg_state := total_map (bitvec 4).
+Definition reg_state := total_map (BITS 32).
 
 Inductive ins : Type :=
 | seq : ins -> ins -> ins
-| mov : reg -> (bitvec 4) -> ins.
+| add : Reg -> Reg -> Reg -> ins
+| mov : Reg -> (BITS 32) -> ins.
 
 Notation "i1 ;; i2" :=
   (seq i1 i2) (at level 80, right associativity).
@@ -59,21 +154,36 @@ Inductive armR : ins -> reg_state -> reg_state -> Prop :=
     armR i1 st st' ->
     armR i2 st' st'' ->
     armR (i1 ;; i2) st st''
-| EMov : forall st st' reg cnst,
-    armR (mov reg cnst) st (t_update st' reg cnst).
+| EAdd : forall rd rn rop2 st,
+    armR (add rd rn rop2) st (t_update st rd
+                               (snd (splitmsb (adcBmain false (st rn) (st rop2)))))
+| EMov : forall st reg cnst,
+    armR (mov reg cnst) st (t_update st reg cnst).
 
 (* ====================================================================== *)
 
 Definition AddLoopArm : ins :=
-  (mov r6 (BEndian _ [true;false;true;false])) ;;
-  (mov r3 (BEndian _ [false;false;false;true])) ;;
-  (mov r6 (BEndian _ [true;false;false;true])).
+  (mov r1 (fromNat 5)) ;;
+  (mov r3 (fromNat 0)) ;;
+  (mov r2 (fromNat 1)) ;;
+  (add r6 r1 r2).
   
 Lemma finalstate8: forall st st' : reg_state,
          (armR AddLoopArm st st') ->
-         st' r6 = BEndian _ [true;false;false;true].
+         (toNat (st' r6)) = 6.
 Proof.
-  unfold AddLoopArm. intros. inversion H. subst.
-  inversion H5. subst. inversion H7. subst. unfold t_update.
+  unfold AddLoopArm. intros. inversion H.
+  inversion H5. inversion H11. inversion H14.
+  inversion H2. inversion H8. subst.
+  inversion H17. rewrite t_update_eq.
+  rewrite t_update_neq. rewrite t_update_eq.
+  rewrite t_update_neq. rewrite t_update_eq.
+  
+  
   reflexivity.
-Qed.
+  
+
+
+  inversion H. subst.
+  inversion H5. subst. inversion H7. subst. inversion H9.
+  subst. inversion H4. subst.
